MathematicalLogic/FirstOrder/Syntax.lean
@@ -2,19 +2,19 @@ import Mathlib.Data.Nat.Basic
 import Mathlib.Data.Set.Basic
 import Mathlib.Order.BoundedOrder
 
-structure Symbol where
+structure Language where
   𝓕 : ℕ → Type
   𝓟 : ℕ → Type
 
-def const (𝓢 : Symbol) := 𝓢.𝓕 0
+def Const (𝓛 : Language) := 𝓛.𝓕 0
 
 mutual
-inductive Term : Symbol → Type where
-| var : ℕ → Term 𝓢
-| func : 𝓢.𝓕 n → Terms 𝓢 n → Term 𝓢
-inductive Terms : Symbol → ℕ → Type where
-| nil : Terms 𝓢 0
-| cons : Term 𝓢 → Terms 𝓢 n → Terms 𝓢 (n + 1)
+inductive Term : Language → Type where
+| var : ℕ → Term 𝓛
+| func : 𝓛.𝓕 n → Terms 𝓛 n → Term 𝓛
+inductive Terms : Language → ℕ → Type where
+| nil : Terms 𝓛 0
+| cons : Term 𝓛 → Terms 𝓛 n → Terms 𝓛 (n + 1)
 end
 
 prefix:max "#" => Term.var
@@ -31,30 +31,32 @@ macro_rules
     expandListLit elems.elemsAndSeps.size false (← ``(Terms.nil))
 
 mutual
-@[simp] def Term.size : Term 𝓢 → ℕ
+@[simp] def Term.size : Term 𝓛 → ℕ
 | #_ => 0
 | _ ⬝ₜ ts => ts.size + 1
-@[simp] def Terms.size : Terms 𝓢 n → ℕ
+@[simp] def Terms.size : Terms 𝓛 n → ℕ
 | []ₜ => 0
 | t ∷ₜ ts => t.size + ts.size + 1
 end
 
 mutual
-def Term.vars : Term 𝓢 → Set ℕ
+def Term.vars : Term 𝓛 → Set ℕ
 | #x => {x}
 | _ ⬝ₜ ts => ts.vars
-def Terms.vars : Terms 𝓢 n → Set ℕ
+def Terms.vars : Terms 𝓛 n → Set ℕ
 | []ₜ => {}
 | t ∷ₜ ts => t.vars ∪ ts.vars
 end
 
-def Subst (𝓢) := ℕ → Term 𝓢
+
+
+def Subst (𝓛) := ℕ → Term 𝓛
 
 mutual
-def Term.subst : Term 𝓢 → Subst 𝓢 → Term 𝓢
+def Term.subst : Term 𝓛 → Subst 𝓛 → Term 𝓛
 | #x, σ => σ x
 | f ⬝ₜ ts, σ => f ⬝ₜ (ts.subst σ)
-def Terms.subst : Terms 𝓢 n → Subst 𝓢 → Terms 𝓢 n
+def Terms.subst : Terms 𝓛 n → Subst 𝓛 → Terms 𝓛 n
 | []ₜ, _ => []ₜ
 | t ∷ₜ ts, σ => t.subst σ ∷ₜ ts.subst σ
 end
@@ -64,7 +66,7 @@ notation:max ts "[" σ "]ₜₛ" => Terms.subst ts σ
 
 theorem Term.subst_ext : σ₁ = σ₂ → t[σ₁]ₜ = t[σ₂]ₜ := by intro h; rw [h]
 
-def Subst.id : Subst 𝓢 := λ x => #x
+def Subst.id : Subst 𝓛 := λ x => #x
 mutual
 theorem Term.subst_id : t[Subst.id]ₜ = t := match t with
 | #x => by rw [Term.subst]; rfl
@@ -74,7 +76,7 @@ theorem Terms.subst_id : ts[Subst.id]ₜₛ = ts := match ts with
 | t ∷ₜ ts => by rw [Terms.subst, Term.subst_id, Terms.subst_id]
 end
 
-def Subst.comp (σ₁ σ₂ : Subst 𝓢) : Subst 𝓢 := λ x => (σ₁ x)[σ₂]ₜ
+def Subst.comp (σ₁ σ₂ : Subst 𝓛) : Subst 𝓛 := λ x => (σ₁ x)[σ₂]ₜ
 infixl:90 " ∘ₛ " => Subst.comp
 mutual
 theorem Term.subst_comp : t[σ₁]ₜ[σ₂]ₜ = t[σ₁ ∘ₛ σ₂]ₜ := match t with
@@ -85,14 +87,17 @@ theorem Terms.subst_comp : ts[σ₁]ₜₛ[σ₂]ₜₛ = ts[σ₁ ∘ₛ σ₂]
 | t ∷ₜ ts => by simp only [Terms.subst]; rw [Term.subst_comp, Terms.subst_comp]
 end
 
-def Subst.single : Term 𝓢 → Subst 𝓢
+def Subst.single : Term 𝓛 → Subst 𝓛
 | t, 0 => t
 | _, x + 1 => #x
 prefix:max "↦ₛ " => Subst.single
 
-def Subst.shift : Subst 𝓢 := λ x => #(x + 1)
-def Term.shift (t : Term 𝓢) := t[Subst.shift]ₜ
+def Subst.shift : Subst 𝓛 := λ x => #(x + 1)
+def Term.shift (t : Term 𝓛) := t[Subst.shift]ₜ
 prefix:max "↑ₜ" => Term.shift
+
+@[simp] theorem shift_of_var : ↑ₜ(#x : Term 𝓛) = #(x+1)
+  := by simp [Term.shift, Term.subst, Subst.shift]
 
 theorem Term.shift_subst_single : (↑ₜt₁)[↦ₛ t₂]ₜ = t₁ := by
   rw [Term.shift, Term.subst_comp]
@@ -150,7 +155,7 @@ theorem Terms.is_shift_iff : (∃ ts', ts = ts'[Subst.shift]ₜₛ) ↔ 0 ∉ ts
     rw [Terms.subst, Term.shift] 
 end
 
-def Subst.lift : Subst 𝓢 → Subst 𝓢
+def Subst.lift : Subst 𝓛 → Subst 𝓛
 | _, 0 => #0
 | σ, x + 1 => ↑ₜ(σ x)
 prefix:max "⇑ₛ" => Subst.lift
@@ -161,7 +166,7 @@ theorem Term.shift_subst_lift : (↑ₜt)[⇑ₛσ]ₜ = ↑ₜ(t[σ]ₜ) := by
   funext x
   rfl
 
-theorem Subst.lift_id : ⇑ₛ(Subst.id : Subst 𝓢) = Subst.id := by
+theorem Subst.lift_id : ⇑ₛ(Subst.id : Subst 𝓛) = Subst.id := by
   funext x
   cases x <;> simp [Subst.lift, Subst.id, Term.shift, Subst.shift, Term.subst]
 
@@ -177,24 +182,23 @@ theorem Subst.lift_comp : ⇑ₛ(σ₁ ∘ₛ σ₂) = ⇑ₛσ₁ ∘ₛ ⇑ₛ
 
 
 
-
-inductive Formula : Symbol → Type where
-| atom : 𝓢.𝓟 n → Terms 𝓢 n → Formula 𝓢
-| false : Formula 𝓢
-| implies : Formula 𝓢 → Formula 𝓢 → Formula 𝓢
-| all : Formula 𝓢 → Formula 𝓢
+inductive Formula : Language → Type where
+| atom : 𝓛.𝓟 n → Terms 𝓛 n → Formula 𝓛
+| false : Formula 𝓛
+| implies : Formula 𝓛 → Formula 𝓛 → Formula 𝓛
+| all : Formula 𝓛 → Formula 𝓛
 
 namespace Formula
-  variable (p q : Formula 𝓢)
+  variable (p q : Formula 𝓛)
   
   infix:70 " ⬝ₚ " => atom
   infixr:55 " ⟶ " => implies
   
-  instance : Bot (Formula 𝓢) where
+  instance : Bot (Formula 𝓛) where
     bot := false
   @[reducible] def neg := p ⟶ ⊥
   prefix:58 "~ " => neg
-  instance : Top (Formula 𝓢) where
+  instance : Top (Formula 𝓛) where
     top := ~ ⊥
   
   @[reducible] def or := ~ p ⟶ q
@@ -209,13 +213,13 @@ namespace Formula
   prefix:59 "∃' " => exist
 end Formula
 
-def Formula.free : Formula 𝓢 → Set ℕ
+def Formula.free : Formula 𝓛 → Set ℕ
 | _ ⬝ₚ ts => ts.vars
 | ⊥ => {}
 | p ⟶ q => p.free ∪ q.free
 | ∀' p => {x | x + 1 ∈ p.free}
 
-def Formula.subst : Formula 𝓢 → Subst 𝓢 → Formula 𝓢
+def Formula.subst : Formula 𝓛 → Subst 𝓛 → Formula 𝓛
 | p ⬝ₚ ts, σ => p ⬝ₚ ts[σ]ₜₛ
 | ⊥, _ => ⊥
 | p ⟶ q, σ => p.subst σ ⟶ q.subst σ
@@ -223,7 +227,7 @@ def Formula.subst : Formula 𝓢 → Subst 𝓢 → Formula 𝓢
 
 notation:80 p "[" σ "]ₚ" => Formula.subst p σ
 
-def Formula.shift : Formula 𝓢 → Formula 𝓢 := λ p => p[Subst.shift]ₚ
+def Formula.shift : Formula 𝓛 → Formula 𝓛 := λ p => p[Subst.shift]ₚ
 prefix:max "↑ₚ" => Formula.shift
 
 theorem Formula.subst_ext : σ₁ = σ₂ → p[σ₁]ₚ = p[σ₂]ₚ := by intro h; rw [h]
